\documentclass[12pt]{article}
\usepackage[legalpaper, margin = 1 in]{geometry}
\usepackage{amsfonts}
\usepackage{amsmath}
\usepackage{graphicx}
\usepackage{graphics}
\usepackage{amssymb}
\usepackage{bm}

\title{HW #4}
\author{Sonny Ji}
\date{ME380}

\begin{document}
\maketitle
\setlength{\parskip}{5pt}


$\\$ 1.a) \dotfill $\\$

$G\left(s\right) = \frac{\left(s + 2\right) \left(s + 5\right)}{s \left(s + 1\right) \left(s + 3\right)}$

The poles of $G\left(s\right)$ are at 0, -1, and -3. Thus, there is only 1 pole at $s = 0$. Thus, for $\frac{Y\left(s\right)}{R\left(s\right)}$, \fbox{the type number is 1}.

$\\$ 1.b) \dotfill $\\$

$e_{ss} \le 0.1$

\begin{quote}

	i) Unit step input
	
	Since $G\left(s\right)$ is a type 1 system, the error of a step input is 0. Thus, \fbox{any $K > 0$} will satisfy the error requirement, since $0 \le 0.1$ is always true.
	
\end{quote}

\begin{quote}

	ii) Unit ramp input

	$e_{ss} = \lim\limits_{s \to 0} s E\left(s\right) = \lim\limits_{s \to 0} \frac{1}{s K G\left(s\right)}$

	$= \lim\limits_{s \to 0} \frac{s \left(s + 1\right) \left(s + 3\right)}{s K \left(s + 2\right) \left(s + 5\right)}$

	$= \lim\limits_{s \to 0} \frac{\left(s + 1\right) \left(s + 3\right)}{K \left(s + 2\right) \left(s + 5\right)}$

	$= \frac{\left(1\right) \left(3\right)}{K \left(2\right) \left(5\right)}$

	$= \frac{3}{10K}$

	$\therefore e_{ss} \le 0.1 \implies \frac{3}{10K} \le 0.1$

	$\therefore$ \fbox{$K \ge 3$}

\end{quote}

\newpage

$\\$ 2.a) \dotfill $\\$

$G\left(s\right) = \frac{200}{s^2 + 20s + 200}$

$G_R\left(s\right) = \frac{Y\left(s\right)}{R\left(s\right)}$

$G_D\left(s\right) = \frac{Y\left(s\right)}{D\left(s\right)}$

$Y\left(s\right) = \left(\left(\left(R\left(s\right) - Y\left(s\right)\right) \cdot \frac{K}{0.1s + 1}\right) + D\left(s\right)\right) \cdot G\left(s\right)$

$Y\left(s\right) = G\left(s\right)\left(R\left(s\right) - Y\left(s\right)\right) \cdot \frac{K}{0.1s + 1} + G\left(s\right)D\left(s\right)$

$Y\left(s\right) + \frac{G\left(s\right)K}{0.1s + 1} \cdot Y\left(s\right) = \frac{G\left(s\right)R\left(s\right)K}{0.1s + 1} + G\left(s\right)D\left(s\right)$

$Y\left(s\right) = \frac{\frac{G\left(s\right)R\left(s\right)K}{0.1s + 1} + G\left(s\right)D\left(s\right)}{1 + \frac{G\left(s\right)K}{0.1s + 1}}$

$Y\left(s\right) = \left(\frac{G\left(s\right)R\left(s\right)K}{0.1s + 1} + G\left(s\right)D\left(s\right)\right) \cdot \frac{0.1s + 1}{0.1s + 1 + G\left(s\right)K}$

$Y\left(s\right) = \frac{G\left(s\right)R\left(s\right)K}{0.1s + 1 + G\left(s\right)K} + \frac{\left(0.1s + 1\right)G\left(s\right)D\left(s\right)}{0.1s + 1 + G\left(s\right)K}$

$Y\left(s\right) = \frac{K}{\frac{0.1s + 1}{\frac{200}{s^2 + 20s + 200}} + K} \cdot R\left(s\right) + \frac{0.1s + 1}{\frac{0.1s + 1}{\frac{200}{s^2 + 20s + 200}} + K} \cdot D\left(s\right)$

$Y\left(s\right) = \frac{K}{\frac{\left(0.1s + 1\right)\left(s^2 + 20s + 200\right)}{200} + K} \cdot R\left(s\right) + \frac{0.1s + 1}{\frac{\left(0.1s + 1\right)\left(s^2 + 20s + 200\right)}{200} + K} \cdot D\left(s\right)$

$Y\left(s\right) = \frac{200K}{0.1s^3 + 2s^2 + 20s + s^2 + 20s + 200 + 200K} \cdot R\left(s\right) + \frac{20s + 200}{0.1s^3 + 2s^2 + 20s + s^2 + 20s + 200 + 200K} \cdot D\left(s\right)$

$Y\left(s\right) = \frac{200K}{0.1s^3 + 3s^2 + 40s + 200 + 200K} \cdot R\left(s\right) + \frac{20s + 200}{0.1s^3 + 3s^2 + 40s + 200 + 200K} \cdot D\left(s\right)$

$Y\left(s\right) = \frac{2000K}{s^3 + 30s^2 + 400s + 2000 + 2000K} \cdot R\left(s\right) + \frac{200s + 2000}{s^3 + 30s^2 + 400s + 2000 + 2000K} \cdot D\left(s\right)$

$\therefore$

\fbox{$G_R\left(s\right) = \frac{2000K}{s^3 + 30s^2 + 400s + 2000 + 2000K}$}

\fbox{$G_D\left(s\right) = \frac{200s + 2000}{s^3 + 30s^2 + 400s + 2000 + 2000K}$}

$\\$ 2.b) \dotfill $\\$

The characteristic equation of $G_R\left(s\right)$ is \fbox{the same} as the characteristic equation of $G_D\left(s\right)$

$\\$ 2.c) \dotfill $\\$

$y_{ss} \le 0.01$

$e_{ss} \le 0.04$

$y_{ss} = \lim\limits_{s \to 0} s Y\left(s\right)$

$e_{ss} = \lim\limits_{s \to 0} s E\left(s\right) = \lim\limits_{s \to 0} s R\left(s\right) - \lim\limits_{s \to 0} s Y\left(s\right)$

$\therefore e_{ss} = \lim\limits_{s \to 0} s R\left(s\right) - y_{ss}$

$r_{ss} = \lim\limits_{s \to 0} s R\left(s\right) = \lim\limits_{t \to \infty} \bm{1}\left(t\right) = 1$

$\therefore e_{ss} = 1 - y_{ss}$

$\therefore 0.04 \ge 1 - y_{ss} \implies 0.96 \le y_{ss} \implies \bot$

Thus, there are \fbox{no values of K} to satisfy both requirements.

\newpage

$\\$ 3.a) \dotfill $\\$

$E\left(s\right) = R\left(s\right) - Y\left(s\right)$

$Y\left(s\right) = \left(K R\left(s\right) - K Y\left(s\right) - B Y\left(s\right)\right) \cdot A \cdot \frac{1}{s}$

$Y\left(s\right) = A \frac{1}{s} K R\left(s\right) - A \frac{1}{s} K Y\left(s\right) - A \frac{1}{s} B Y\left(s\right)$

$Y\left(s\right) \left(1 + \frac{AK}{s} + \frac{AB}{s}\right) = \frac{AK}{s} R\left(s\right)$

$Y\left(s\right) = \frac{AK}{s + AK + AB} R\left(s\right)$

$\therefore E\left(s\right) = R\left(s\right) - \frac{AK}{s + AK + AB} R\left(s\right)$

$= R\left(s\right) \left(1 - \frac{AK}{s + AK + AB}\right)$

$= R\left(s\right) \frac{s + AB}{s + AK + AB}$

$\therefore$ \fbox{$G_E\left(s\right) = \frac{s + AB}{s + AK + AB}$}

$\\$ 3.b) \dotfill $\\$

$E\left(s\right) = G_E\left(s\right) R\left(s\right)$

$r\left(t\right) = 2 \cdot \bm{1}\left(t\right)$

$R\left(s\right) = \frac{2}{s}$

$E\left(s\right) = \frac{s + AB}{s + AK + AB} \cdot \frac{2}{s}$

$e_{ss} = \lim\limits_{s \to 0} sE\left(s\right)$

$= \lim\limits_{s \to 0} \frac{s + AB}{s + AK + AB} \cdot 2$

$\therefore$ \fbox{$e_{ss} = \frac{2B}{K + B}$}

$\\$ 3.c) \dotfill $\\$

$r\left(t\right) = 2 t \cdot \bm{1}\left(t\right)$

$R\left(s\right) = \frac{2}{s^2}$

$E\left(s\right) = \frac{s + AB}{s + AK + AB} \cdot \frac{2}{s^2}$

$e_{ss} = \lim\limits_{s \to 0} \frac{s + AB}{s + AK + AB} \cdot \frac{2}{s}$

$= \lim\limits_{s \to 0} \frac{2s + 2AB}{s^2 + AKs + ABs}$

$= \frac{2AB}{0}$

$\therefore$ \fbox{$e_{ss} = \infty$}

$\\$ 3.d) \dotfill $\\$

$r\left(t\right) = 2 t^2 \cdot \bm{1}\left(t\right)$

$R\left(s\right) = \frac{4}{s^3}$

$E\left(s\right) = \frac{s + AB}{s + AK + AB} \cdot \frac{4}{s^3}$

$e_{ss} = \lim\limits_{s \to 0} \frac{s + AB}{s + AK + AB} \cdot \frac{4}{s^2}$

$= \lim\limits_{s \to 0} \frac{4s + 4AB}{s^3 + AKs^2 + ABs^2}$

$= \frac{4AB}{0}$

$\therefore$ \fbox{$e_{ss} = \infty$}

\newpage

$\\$ 4.a) \dotfill $\\$

$G\left(s\right) = \frac{1}{s + 2}$

$G_c\left(s\right) = \frac{K}{s + 10}$

\begin{quote}

	i)

	The open-loop transfer function $G\left(s\right) G_c\left(s\right)$ is $\frac{K}{\left(s + 2\right) \left(s + 10\right)}$ which has no poles at $s = 0$, thus the system is \fbox{type number 0}.

\end{quote}

\begin{quote}

	ii)

	$e_{ss} \le 0.2$

	Since the system is type 0, the response to a step input is:
	
	$e_{ss} = \lim\limits_{s \to 0} \frac{1}{1 + G\left(s\right) G_c\left(s\right)}$

	$= \lim\limits_{s \to 0} \frac{1}{1 + \frac{K}{\left(s + 2\right) \left(s + 10\right)}}$

	$= \lim\limits_{s \to 0} \frac{\left(s + 2\right) \left(s + 10\right)}{\left(s + 2\right) \left(s + 10\right) + K}$

	$= \frac{\left(2\right) \left(10\right)}{\left(2\right) \left(10\right) + K}$

	$= \frac{20}{20 + K}$

	$\therefore 0.2 \ge \frac{20}{20 + K} \implies$ \fbox{$80 \le K$}

\end{quote}

$\\$ 4.b) \dotfill $\\$

$G_c\left(s\right) = \frac{K}{s \left(s + 10\right)}$

\begin{quote}

	i)

	The open-loop transfer function $G\left(s\right) G_c\left(s\right)$ is $\frac{K}{s \left(s + 2\right) \left(s + 10\right)}$ which has one poles at $s = 0$, thus the system is \fbox{type number 1}.

\end{quote}

\begin{quote}

	ii)

	$e_{ss} \le 0.2$

	Since the system is type 1, the response to a step input is 0. Thus, since $0 \le 0.2$ is always true, \fbox{any $K > 0$} will satisfy the requirement.

\end{quote}

$\\$ 4.c) \dotfill $\\$

\begin{quote}

	i)

	For $G_c\left(s\right) = \frac{K}{s + 10}$:

	$\frac{Y\left(s\right)}{R\left(s\right)} = \frac{G\left(s\right) G_c\left(s\right)}{1 + G\left(s\right) G_c\left(s\right)}$

	$= \frac{\frac{K}{\left(s + 2\right) \left(s + 10\right)}}{1 + \frac{K}{\left(s + 2\right) \left(s + 10\right)}}$

	$= \frac{1}{\frac{\left(s + 2\right) \left(s + 10\right)}{K} + 1}$

	$= \frac{K}{\left(s + 2\right) \left(s + 10\right) + K}$

	$=$ \fbox{$\frac{K}{s^2 + 12s + 20 + K}$}

	For $G_c\left(s\right) = \frac{K}{s \left(s + 10\right)}$:

	$\frac{Y\left(s\right)}{R\left(s\right)} = \frac{\frac{K}{s \left(s + 2\right) \left(s + 10\right)}}{1 + \frac{K}{s \left(s + 2\right) \left(s + 10\right)}}$

	$= \frac{1}{\frac{s \left(s + 2\right) \left(s + 10\right)}{K} + 1}$

	$= \frac{K}{s \left(s + 2\right) \left(s + 10\right) + K}$

	$=$ \fbox{$\frac{K}{s^3 + 12s^2 + 20s + K}$}

\end{quote}

\begin{quote}

	ii)

	Attached at end.

\end{quote}

$\\$ 4.d) \dotfill $\\$

The system with $G_c\left(s\right) = \frac{K}{s \left(s + 10\right)}$ has better steady-state performance, since the output settles to 1, meaning the error is 0, while the system with $G_c\left(s\right) = \frac{K}{s + 10}$ always has an offset in the output. This matches the steady-state error results from (b).


\end{document}